theories/tactic.v
@@ -1,5 +1,5 @@
 From mathcomp Require Import ssreflect ssrfun ssrnat ssrbool eqtype seq.
-From Wasm Require Import typing_inversion.
+From Wasm Require Import properties typing_inversion.
 
 Ltac size_unequal H :=
   repeat rewrite length_is_size in H;
@@ -62,3 +62,164 @@ Ltac solve_progress_cont cont :=
 (** The same, but without continuation. **)
 Ltac solve_progress :=
   solve_progress_cont ltac:(fail).
+
+
+(* Looking up from instances, stores, and contexts *)
+Ltac inst_typing_lookup :=
+  try multimatch goal with
+  | H1: inst_typing ?s ?i = Some ?t,
+    H2: lookup_N (inst_types ?i) ?n = Some _ |- _ =>
+      let Hteq := fresh "Hteq" in
+      specialize (Logic.eq_sym (inst_typing_type_lookup n H1)) as Hteq;
+      rewrite H2 in Hteq
+  | H1: inst_typing ?s ?i = Some ?t,
+    H2: lookup_N (inst_funcs ?i) _ = Some _ |- _ =>
+      let ft := fresh "ft" in
+      let Hextft := fresh "Hextft" in
+      let Hnthft := fresh "Hnthft" in
+      specialize (inst_typing_func_lookup H1 H2) as [ft [Hextft Hnthft]];
+      unfold ext_func_typing in Hextft
+  | H1: inst_typing ?s ?i = Some ?t,
+    H2: lookup_N (inst_tables ?i) _ = Some _ |- _ =>
+      let tabt := fresh "tabt" in
+      let Hexttabt := fresh "Hexttabt" in
+      let Hnthtabt := fresh "Hnthtabt" in
+      specialize (inst_typing_table_lookup H1 H2) as [tabt [Hexttabt Hnthtabt]];
+      unfold ext_table_typing in Hexttabt
+  | H1: inst_typing ?s ?i = Some ?t,
+    H2: lookup_N (inst_mems ?i) _ = Some _ |- _ =>
+      let mt := fresh "mt" in
+      let Hextmt := fresh "Hextmt" in
+      let Hnthmt := fresh "Hnthmt" in
+      specialize (inst_typing_mem_lookup H1 H2) as [mt [Hextmt Hnthmt]];
+      unfold ext_mem_typing in Hextmt
+  | H1: inst_typing ?s ?i = Some ?t,
+    H2: lookup_N (inst_globals ?i) _ = Some _ |- _ =>
+      let gt := fresh "gt" in
+      let Hextgt := fresh "Hextgt" in
+      let Hnthgt := fresh "Hnthgt" in
+      specialize (inst_typing_global_lookup H1 H2) as [gt [Hextgt Hnthgt]];
+      unfold ext_global_typing in Hextgt
+  | H1: inst_typing ?s ?i = Some ?t,
+    H2: lookup_N (inst_elems ?i) _ = Some _ |- _ =>
+      let et := fresh "et" in
+      let ei := fresh "ei" in
+      let Hnthselem := fresh "Hnthselem" in
+      let Helemtype := fresh "Helemtype" in
+      let Hnthet := fresh "Hnthet" in
+      specialize (inst_typing_elem_lookup H1 H2) as [et [ei [Hnthselem [Helemtype Hnthet]]]]
+  | H1: inst_typing ?s ?i = Some ?t,
+    H2: lookup_N (inst_datas ?i) _ = Some _ |- _ =>
+      let dt := fresh "et" in
+      let di := fresh "di" in
+      let Hnthsdata := fresh "Hnthsdata" in
+      let Hdatatype := fresh "Hdatatype" in
+      let Hnthdt := fresh "Hnthdt" in
+      specialize (inst_typing_data_lookup H1 H2) as [dt [di [Hnthsdata [Hdatatype Hnthdt]]]]
+  end.
+
+Ltac store_typing_lookup :=
+  try multimatch goal with
+  | H1: store_typing ?s,
+      H2: lookup_N (s_funcs ?s) _ = Some _ |- _ =>
+      let ft := fresh "ft" in
+      let Hft := fresh "Hft" in
+      specialize (store_typing_func_lookup H1 H2) as [ft Hft];
+      unfold funcinst_typing in Hft
+  | H1: store_typing ?s,
+      H2: lookup_N (s_tables ?s) _ = Some _ |- _ =>
+      let tabt := fresh "tabt" in
+      let Htabt := fresh "Htabt" in
+      specialize (store_typing_table_lookup H1 H2) as [tabt Htabt];
+      unfold tableinst_typing in Htabt
+  | H1: store_typing ?s,
+      H2: lookup_N (s_mems ?s) _ = Some _ |- _ =>
+      let mt := fresh "mt" in
+      let Hmt := fresh "Hmt" in
+      specialize (store_typing_mem_lookup H1 H2) as [mt Hmt];
+      unfold meminst_typing in Hmt
+  | H1: store_typing ?s,
+      H2: lookup_N (s_globals ?s) _ = Some _ |- _ =>
+      let gt := fresh "gt" in
+      let Hgt := fresh "Hgt" in
+      specialize (store_typing_global_lookup H1 H2) as [gt Hgt];
+      unfold globalinst_typing in Hgt
+  | H1: store_typing ?s,
+      H2: lookup_N (s_elems ?s) _ = Some _ |- _ =>
+      let et := fresh "et" in
+      let Het := fresh "Het" in
+      specialize (store_typing_elem_lookup H1 H2) as [et Het];
+      unfold eleminst_typing in Het
+  | H1: store_typing ?s,
+      H2: lookup_N (s_datas ?s) _ = Some _ |- _ =>
+      let dt := fresh "dt" in
+      let Hdt := fresh "Hdt" in
+      specialize (store_typing_data_lookup H1 H2) as [dt Hdt];
+      unfold datainst_typing in Hdt
+  end.
+
+Ltac resolve_store_inst_lookup :=
+  store_typing_lookup; inst_typing_lookup.
+
+Ltac unfold_store_operations :=
+  repeat match goal with
+    | _: context [ stab_update _ _ _ _ ] |- _ =>
+        remove_bools_options
+    | _: context [ supdate_glob _ _ _ _ ] |- _ =>
+        unfold supdate_glob, supdate_glob_s, sglob_ind, option_bind, option_map in *; remove_bools_options
+    | _: context [ sglob_val _ _ ] |- _ =>
+        unfold sglob_val, sglob, sglob_ind in *; remove_bools_options
+    | _: context [ stab_elem _ _ ] |- _ =>
+        unfold stab_elem in *; remove_bools_options
+    | _: context [ stab _ _ ] |- _ =>
+        unfold stab in *; remove_bools_options
+    | _: context [ smem _ _ ] |- _ =>
+        unfold smem in *; remove_bools_options
+    | _: context [ selem _ _ ] |- _ =>
+        unfold selem in *; remove_bools_options
+    | _: context [ sdata _ _ ] |- _ =>
+        unfold sdata in *; remove_bools_options
+    | _: context [ selem_drop _ _ _ ] |- _ =>
+        unfold selem_drop, selem in *; remove_bools_options
+    | _: context [ sdata_drop _ _ _ ] |- _ =>
+        unfold sdata_drop, sdata in *; remove_bools_options
+    end.
+
+Ltac resolve_e_typing :=
+  repeat lazymatch goal with
+    | _ : _ |- e_typing _ _ nil (Tf _ _) =>
+        apply et_empty
+    | _ : _ |- e_typing _ _ _ (Tf ?x (?x ++ _)) =>
+        apply et_weakening_empty_1
+    | H : value_ref_typing ?s ?tabv = Some ?t |-
+        e_typing ?s _ (cons ($V (VAL_ref ?tabv)) nil) (Tf ?ts1 _) =>
+        try apply et_weakening_empty_1; apply et_value_typing => /=; rewrite H => //=
+    | H : value_typing ?s ?v = Some ?t |-
+        e_typing ?s _ (cons ($V ?v) nil) (Tf ?ts1 _) =>
+        try apply et_weakening_empty_1; apply et_value_typing => //=
+    | H : value_ref_typing ?s ?tabv = Some ?t |-
+        e_typing ?s _ (cons ($V (VAL_ref ?tabv)) ?l) (Tf ?ts1 _) =>
+        rewrite -(cat1s ($V (VAL_ref tabv)) l); apply et_composition' with (t2s := ts1 ++ [::T_ref t]); first by try apply et_weakening_empty_1; apply et_value_typing => /=; rewrite H => //=
+    | H : value_typing ?s ?v = Some ?t |-
+        e_typing ?s _ (cons ($V ?v) ?l) (Tf ?ts1 _) =>
+        rewrite -(cat1s ($V v) l); apply et_composition' with (t2s := ts1 ++ [::t]); first by try apply et_weakening_empty_1; apply et_value_typing => //=
+    | _ : value_typing ?s ?v = Some ?t |-
+        e_typing ?s _ [::($V ?v)] (Tf ?ts1 _) =>
+        try apply et_weakening_empty_1; try by apply et_value_typing; eauto => /=
+    | _ : _ |- e_typing _ _ (cons ($VN ?x) _) (Tf _ _) =>
+        replace ($VN x) with ($V (VAL_num x)); last done
+    | _ : _ |- e_typing  _ _ (cons (vref_to_e ?x) _) (Tf _ _) =>
+        replace (vref_to_e x) with ($V (VAL_ref x)); last done
+    | _ : _ |- e_typing _ _ [:: $V _] (Tf nil _) =>
+        try apply et_value_typing => //=
+    | _ : _ |- e_typing _ _ [:: $V _] (Tf ?x ?y) =>
+        try apply et_weakening_empty_1; first by apply et_value_typing => //= 
+    | _ : _ |- e_typing _ _ (cons ($V (VAL_num ?v)) ?l) (Tf ?ts1 _) =>
+        rewrite -(cat1s ($V (VAL_num v)) l); apply et_composition' with (t2s := ts1 ++ [::T_num (typeof_num v)]); eauto; first by try apply et_weakening_empty_1; apply et_value_typing; eauto => //=
+    | _ : _ |- e_typing _ _ (v_to_e_list _) (Tf _ _) =>
+        try apply et_values_typing => /=
+    | H : is_true (const_list _) |- _ =>
+        let vs := fresh "vs" in
+        apply const_es_exists in H as [vs ->]; invert_e_typing
+    | _ => unfold_store_operations
+    end.
